Restructure monad stacks, add reader monad and monad classes

hygiene.lean
@@ -2,8 +2,9 @@ import macro
 
 def α_conv (rsm : resolve_map) (σ : syntax_id → name) : syntax → syntax
 | (syntax.ident ident) := match rsm.find ident.id with
-  | some r := syntax.ident {ident with sp := none, name := ident.name.replace_prefix' r.prefix (σ r.decl)}
-  | none   := syntax.ident {ident with sp := none, name := σ ident.id}
+  -- TODO: renaming of globals?
+  | some r@{decl := sum.inl id, ..} := syntax.ident {ident with sp := none, name := ident.name.replace_prefix' r.prefix (σ id)}
+  | _   := syntax.ident {ident with sp := none, name := σ ident.id}
   end
 | (syntax.node node) := syntax.node {node with args := node.args.map (λ a, α_conv a)}
 | (syntax.list ls) := syntax.list (ls.map (λ a, α_conv a))
@@ -13,12 +14,14 @@ using_well_founded { dec_tac := tactic.admit }
 def α_equiv (rsm : resolve_map) (s₁ s₂ : syntax) :=
 ∃ σ, α_conv rsm σ s₁ = s₂
 
-section
-parameter (macros : name → option macro)
+protected def except.assert {ε} : except ε Prop → Prop
+| (except.ok p)    := p
+| (except.error _) := false
 
-theorem hygienic (s₁ s₂ : syntax) :
-match resolve' macros (expand' macros s₁) : _ → Prop with
-| except.ok (_, rsm) := α_equiv rsm s₁ s₂ → α_equiv rsm (expand' macros s₁) (expand' macros s₂)
-| except.error _ := false
-end := sorry
-end
+theorem hygienic (s₁ s₂ : syntax) (st : parse_state) :
+except.assert $ reader_t.run st $
+(do s₁' ← expand' s₁,
+    s₂' ← expand' s₂,
+    (_, rst) ← resolve' s₁',
+    pure $ α_equiv rst.resolve_map s₁ s₂ → α_equiv rst.resolve_map s₁' s₂')
+:= sorry
