macro.lean
@@ -5,18 +5,28 @@ open state
 
 attribute [instance] name.has_lt_quick option.has_lt
 
+--@[reducible] def parse_m (r σ) := reader_t r $ state_t σ $ except string
+
 structure resolved :=
-(decl : syntax_id)
+-- local or global
+(decl : syntax_id ⊕ name)
 /- prefix of the reference that corresponds to the decl. All trailing name components
    are field accesses. -/
 («prefix» : name)
 
 meta instance : has_to_format resolved := ⟨λ r, to_fmt (r.decl, r.prefix)⟩
 
+structure resolve_cfg :=
+(global_scope : rbmap name syntax)
+
 @[reducible] def resolve_map := rbmap syntax_id resolved
+
+structure resolve_state :=
+(resolve_map : resolve_map)
+
 def scope := rbmap (name × option macro_scope_id) syntax_id
 
-@[reducible] def resolve_m := state_t resolve_map (except string)
+@[reducible] def resolve_m := reader_t resolve_cfg $ state_t resolve_state $ except string
 
 def exp_fuel := 1000
 
@@ -28,19 +38,22 @@ structure macro :=
 (resolve : option (scope → syntax_node syntax → resolve_m (list scope)) := none)
 -- (elaborate : list syntax → expr → tactic expr)
 
+structure parse_state :=
+(macros : rbmap name macro)
+(resolve_cfg : resolve_cfg)
+
+@[reducible] def parse_m := state_t parse_state id
+
 -- identifiers in macro expansions are annotated with incremental tags
 structure expand_state :=
 (next_tag : ℕ)
 
-@[reducible] def exp_m := state expand_state
+@[reducible] def exp_m := reader_t parse_state $ state_t expand_state $ except string
 
 def mk_tag : exp_m ℕ :=
 do st ← read,
    write {st with next_tag := st.next_tag + 1},
    pure st.next_tag
-
-section
-parameter (macros : name → option macro)
 
 def flip_tag (tag : ℕ) : syntax → syntax
 | (syntax.node node) := syntax.node {node with args := (node.args.map
@@ -57,7 +70,8 @@ using_well_founded { dec_tac := tactic.admit } -- TODO
 
 def expand : ℕ → syntax → exp_m syntax
 | (fuel + 1) (syntax.node node) :=
-do some {expand := some exp, ..} ← pure $ macros node.m
+do cfg ← reader_t.read,
+   some {expand := some exp, ..} ← pure $ cfg.macros.find node.m
      | (λ args, syntax.node {node with args := args}) <$> node.args.mmap (expand fuel),
    tag ← mk_tag,
    let node := {node with args := node.args.map $ flip_tag tag},
@@ -65,22 +79,27 @@ do some {expand := some exp, ..} ← pure $ macros node.m
    expand fuel $ flip_tag tag $ exp node
 | _ stx := pure stx
 
-def resolve : scope → syntax → resolve_m unit
+@[reducible] def resolve_m' := reader_t parse_state $ state_t resolve_state $ except string
+
+--instance (r r' m α) [monad m] [has_coe r' r] : has_coe (reader_t r m α) (reader_t r' m α) :=
+--⟨λ x r, x r⟩
+
+def resolve : scope → syntax → resolve_m' unit
 | sc (syntax.node node) :=
-do some {resolve := some res, ..} ← pure $ macros node.m
+do cfg ← reader_t.read,
+   some {resolve := some res, ..} ← pure $ cfg.macros.find node.m
      | node.args.mmap' $ resolve sc,
-   arg_scopes ← res sc node,
+   arg_scopes ← with_reader_t parse_state.resolve_cfg $ res sc node,
    (arg_scopes.zip node.args).mmap' -- (uncurry resolve)
                                     (λ ⟨sc, stx⟩, resolve sc stx)
 | _ _ := pure ()
 using_well_founded { dec_tac := tactic.admit }
 
-def expand' (stx : syntax) : syntax :=
-(expand 1000 stx {next_tag := 0}).1
+def expand' (stx : syntax) : reader_t parse_state (except string) syntax :=
+map_reader_t (λ st, prod.fst <$> state_t.run {expand_state . next_tag := 0} st) (expand 1000 stx)
 
-def resolve' (stx : syntax) : except string (syntax × resolve_map) :=
+def resolve' (stx : syntax) : reader_t parse_state (except string) (syntax × resolve_state) :=
 let sc : scope := mk_rbmap _ _ _,
-    resolve_map : resolve_map := mk_rbmap _ _ _ in
-    do ⟨(), rsm⟩ ← resolve sc stx resolve_map,
+    st : resolve_state := ⟨mk_rbmap _ _ _⟩ in
+    do ⟨(), rsm⟩ ← map_reader_t (state_t.run st) $ resolve sc stx,
        pure (stx, rsm)
-end
