examples.lean
@@ -1,23 +1,20 @@
 import macro
 import hygiene
 
-open except
-
 def sp : option span := none
 
 def lambda_macro := {macro .
   name := "lambda",
   resolve := some $ λ sc node,
   do [syntax.ident ident, body] ← pure node.args
-       -- TODO: add `monad_error` class to remove lift (also, `monad_lift` seems to be broken)
-       | state_t.lift unreachable,
+       | unreachable,
      pure [sc, sc.insert (ident.name, ident.msc) ident.id]}
 
 def resolve_name (msc : option macro_scope_id) (sc : scope) : name → option resolved
 | (name.mk_string s n) :=
 do {
   decl ← sc.find (n.mk_string s, msc),
-  pure ⟨decl, n.mk_string s⟩
+  pure ⟨sum.inl decl, n.mk_string s⟩
 } <|> resolve_name n
 | _ := none
 
@@ -25,10 +22,10 @@ def ref_macro := {macro .
   name := "ref",
   resolve := some $ λ sc node,
   do [syntax.ident ident] ← pure node.args
-       | state_t.lift unreachable,
+       | unreachable,
      some resolved ← pure $ resolve_name ident.msc sc ident.name
-       | state_t.lift $ error sformat!"unknown identifier {ident.name}",
-     state_t.modify (λ h, h.insert ident.id resolved),
+       | fail sformat!"unknown identifier {ident.name}",
+     modify (λ st, ⟨st.resolve_map.insert ident.id resolved⟩),
      pure []}
 
 def intro_x_macro := {macro .
@@ -43,10 +40,14 @@ def macros : name → option macro
 | "intro_x" := some intro_x_macro
 | _ := none
 
+def cfg : parse_state :=
+{macros := rbmap.from_list $ [lambda_macro, ref_macro, intro_x_macro].map (λ m, (m.name, m)),
+ resolve_cfg := {global_scope := mk_rbmap _ _}}
+
 meta def test (stx : syntax) : command :=
-match resolve' macros (expand' macros stx) with
+match (expand' stx >>= resolve') cfg with
 | except.error e := tactic.fail e
-| except.ok    o := tactic.trace stx >> tactic.trace o
+| except.ok    (stx, ⟨rsm⟩) := tactic.trace stx >> tactic.trace (stx, rsm)
 end
 
 run_cmd test $ syntax.node ⟨0, sp, "lambda", [
@@ -82,7 +83,7 @@ let stx := syntax.node ⟨0, sp, "lambda", [
     syntax.ident ⟨3, sp, `x.y.z, none⟩
   ]⟩
 ]⟩ in
-match resolve' macros (expand' macros stx) with
-| except.ok (_, rsm) := tactic.trace (α_conv rsm (λ id, if id = 1 then `a else `b) stx)
+match (expand' stx >>= resolve') cfg with
+| except.ok (_, ⟨rsm⟩) := tactic.trace (α_conv rsm (λ id, if id = 1 then `a else `b) stx)
 | except.error _ := tactic.skip
 end
